cleanup; fix cal_sum

dataset/Dafny/textbook_algo_unit_tests/run_all_py.py
@@ -1,4 +1,0 @@
-import os
-output = os.system("ls")
-glb 
-print("output"+output)
